failed attempt at dbidxing

LeanScratch/LogicProof/FirstOrderLogic/Formula.lean
@@ -18,3 +18,140 @@ inductive Formula {TNm PNm : Type} (TA : TNm → Nat) (PA : PNm → Nat)
   | iff  : Formula TA PA → Formula TA PA → Formula TA PA 
   | neg  : Formula TA PA → Formula TA PA
 
+
+inductive DeBrujin.Term {Nm : Type} (Arity : Nm → Nat) (n : Nat)
+  | const (nm : Nm) (app : Vec (Term Arity n) (Arity nm))
+  | var (v : Fin n)
+
+inductive DeBrujin.Formula {TNm PNm : Type} (TA : TNm → Nat) (PA : PNm → Nat) : Nat → Type
+  | pred (nm : PNm) (app : Vec (Term TA n) (PA nm)) : Formula TA PA n
+
+  | univ : Formula TA PA n.succ → Formula TA PA n
+  | exis : Formula TA PA n.succ → Formula TA PA n
+
+  | conj : Formula TA PA n → Formula TA PA n → Formula TA PA n
+  | disj : Formula TA PA n → Formula TA PA n → Formula TA PA n
+  | imp  : Formula TA PA n → Formula TA PA n → Formula TA PA n
+  | iff  : Formula TA PA n → Formula TA PA n → Formula TA PA n
+  | neg  : Formula TA PA n → Formula TA PA n
+
+def Term.toDeBrujin (t : Term TA) : DeBrujin.Term TA 0 :=
+  match t with
+  | .const nm args => .const nm (mapper args)
+    where
+      mapper {k} : Vec (Term TA) k → Vec _ k
+        | %[] => %[]
+        | hd %:: tl => hd.toDeBrujin %:: mapper tl
+
+namespace DeBrujin
+
+def Term.subst (pt : Fin n.succ) (body : Term TA n.succ) (repl : Term TA n) : Term TA n :=
+  match body with
+  | .var ⟨x, p⟩ => match h : compare x pt.val with
+    | .lt =>
+      have xSuccLe := Nat.compare_eq_lt.mp h
+      .var ⟨x, by omega⟩
+    | .eq => repl
+    | .gt =>
+      have xSuccLe := Nat.compare_eq_gt.mp h
+      .var ⟨x - 1, by omega⟩
+  | .const nm args => .const nm (mapper args)
+    where
+      mapper {k} : Vec (Term TA n.succ) k → Vec (Term TA n) k
+        | %[] => %[]
+        | hd %:: tl => (hd.subst pt repl) %:: mapper tl
+
+def Term.bvarShift (k : Nat) : Term TA n → Term TA (n + k)
+  | .var v => .var $ v.addNat k
+  | .const nm args => .const nm (mapper args)
+    where
+      mapper {m} : Vec (Term TA n) m → Vec (Term TA (n + k)) m
+        | %[] => %[]
+        | hd %:: tl => (hd.bvarShift k) %:: mapper tl
+
+def Formula.subst
+    (pt : Fin n.succ) (body : Formula TA PA n.succ)
+    (repl : Term TA n) : Formula TA PA n :=
+  match body with
+  | .pred nm app => .pred nm (Term.subst.mapper pt repl app)
+
+  | .univ p => .univ $ p.subst pt $ repl.bvarShift 1
+  | .exis p => .exis $ p.subst pt $ repl.bvarShift 1
+
+  | .conj a b => .conj (a.subst pt repl) (b.subst pt repl)
+  | .disj a b => .disj (a.subst pt repl) (b.subst pt repl)
+  | .imp a b => .imp (a.subst pt repl) (b.subst pt repl)
+  | .iff a b => .iff (a.subst pt repl) (b.subst pt repl)
+  | .neg v => .neg $ v.subst pt repl
+
+theorem substAllEq {m : ℕ} {offset n : ℕ} : offset < offset + m + n + 1 := by
+  apply Nat.lt_add_one_of_le
+  omega
+
+def Term.substAll (offset : Nat) (int : Term TA (offset + m + n)) : Vec (Term TA (offset + m)) n → Term TA (offset + m)
+  | hd %:: tl => (int.subst ⟨offset, substAllEq⟩ (hd.bvarShift _)).substAll offset tl
+  | %[] => int
+
+def Formula.substAll (offset : Nat) (inf : Formula TA PA (offset + m + n)) : Vec (Term TA (offset + m)) n → Formula TA PA (offset + m)
+  | hd %:: tl => (inf.subst ⟨offset, substAllEq⟩ (hd.bvarShift _)).substAll offset tl
+  | %[] => inf
+
+def Term.toHoAS (t : Term TA 0) : FOL.Term TA :=
+  match t with
+  | .var v => v.elim0
+  | .const nm args => .const nm (mapper args)
+    where
+      mapper {k} : Vec (Term TA 0) k → Vec _ k
+        | %[] => %[]
+        | hd %:: tl => hd.toHoAS %:: mapper tl
+
+def Formula.sz : Formula TA PA n → Nat
+  | .pred _ _ => 1
+
+  | .neg p 
+  | .univ p 
+  | .exis p => p.sz + 1
+
+  | .conj a b
+  | .disj a b
+  | .imp a b
+  | .iff a b => a.sz + b.sz + 1
+
+theorem Formula.subst.sz
+    {repl : Term TA n} {f : Formula TA PA n.succ}
+    : (f.subst pt repl).sz = f.sz :=
+  match f with
+  | .pred _ _ => by simp only [subst]; rfl
+
+  | .neg p
+  | .univ p
+  | .exis p => by
+    simp only [subst]
+    change _ + 1 = _ + 1
+    rw [Formula.subst.sz]
+  | .conj a b
+  | .disj a b
+  | .imp a b
+  | .iff a b => by
+    simp only [subst]
+    change _ + 1 = _ + 1
+    rw [Formula.subst.sz, Formula.subst.sz]
+
+def Formula.toHoAS : Formula TA PA 0 → FOL.Formula TA PA
+  | .pred nm app => .pred nm (Term.toHoAS.mapper app)
+
+  | .univ p => .univ fun x => (p.subst ⟨0, Nat.zero_lt_succ _⟩ x.toDeBrujin).toHoAS
+  | .exis p => .exis fun x => (p.subst ⟨0, Nat.zero_lt_succ _⟩ x.toDeBrujin).toHoAS
+
+  | .conj a b => .conj a.toHoAS b.toHoAS
+  | .disj a b => .disj a.toHoAS b.toHoAS
+  | .imp  a b => .imp  a.toHoAS b.toHoAS
+  | .iff  a b => .iff  a.toHoAS b.toHoAS
+  | .neg v => .neg v.toHoAS
+termination_by f => f.sz
+decreasing_by
+all_goals simp_wf
+all_goals (try { dsimp [sz]; omega })
+all_goals rw [subst.sz]
+all_goals exact Nat.lt_succ_self _
+
