LeanScratch/LogicProof/FirstOrderLogic/DenseFormula.lean
@@ -1,0 +1,62 @@
+import LeanScratch.Vec
+import LeanScratch.LogicProof.FirstOrderLogic.Formula
+
+
+namespace FOL.DeBrujin
+
+inductive Dense.Base {TNm PNm : Type} (TA : TNm → Nat) (PA : PNm → Nat) (n : Nat)
+  | pred  (nm : PNm) (app : Vec (Term TA n) (PA nm)) : Base TA PA n
+  | npred (nm : PNm) (app : Vec (Term TA n) (PA nm)) : Base TA PA n
+
+  | conj : Base TA PA n → Base TA PA n → Base TA PA n
+  | disj : Base TA PA n → Base TA PA n → Base TA PA n
+
+def Dense.Base.bvarShift (k : Nat) : Base TA PA n → Base TA PA (n + k)
+  | .pred nm app => .pred nm $ Term.bvarShift.mapper _ app
+  | .npred nm app => .pred nm $ Term.bvarShift.mapper _ app
+  | .disj a b => .disj (a.bvarShift k) (b.bvarShift k)
+  | .conj a b => .conj (a.bvarShift k) (b.bvarShift k)
+
+inductive Dense {TNm PNm : Type} (TA : TNm → Nat) (PA : PNm → Nat) : Nat → Type
+  | bot : Dense.Base TA PA n → Dense TA PA n
+  | exis : Dense TA PA n.succ → Dense TA PA n
+  | univ : Dense TA PA n.succ → Dense TA PA n
+
+def Dense.conjunctiveTransform : Dense TA PA n → Dense TA PA (n + k) → Dense TA PA (n + k)
+  | .bot x, .bot y  => .bot (.conj (x.bvarShift k) y)
+  | x, .univ y => .univ (conjunctiveTransform (k := k + 1) x y)
+  | x, .exis y => .exis (conjunctiveTransform (k := k + 1) x y)
+  | .exis x, y => match k with
+    | 0 => .exis $ conjunctiveTransform (n := n) (k := 1) y x
+    | k+1 =>
+      /- have : Dense TA PA := sorry -/
+      .exis sorry
+  | .univ x, y => sorry
+  /- | .univ x, .univ y => .univ $ conjunctiveTransform x y -/
+  /- | y, .univ x | .univ x, y => .univ fun v => conjunctiveTransform (x v) y -/
+  /- | y, .exis x | .exis x, y => .exis fun v => conjunctiveTransform (x v) y -/
+
+-- Since n represents free varaibles this will always be the same but the way
+-- these are bound by quiantifiers will strictly vary due to how PNX NF works
+def Formula.transform : Bool → Formula TA PA n → Dense TA PA n
+  | .true, .pred nm app  => .bot $ .pred nm app
+  | .false, .pred nm app => .bot $ .npred nm app
+
+  | .true,  .conj a b => sorry-- conjunctiveTransform (a.transform .true) (b.transform .true)
+  | .false, .conj a b => sorry
+  | .true,  .disj a b => sorry
+  | .false, .disj a b => sorry
+  | .true,  .imp a b  => sorry
+  | .false, .imp a b  => sorry
+  | .true,  .iff a b  => sorry
+  | .false, .iff a b  => sorry
+  | .true,  .neg v    => v.transform .false
+  | .false, .neg v    => v.transform .true
+
+  | .true,  .exis v => .exis $ v.transform .true
+  | .true,  .univ v => .univ $ v.transform .true
+  | .false, .exis v => .univ $ v.transform .false
+  | .false, .univ v => .exis $ v.transform .false
+
+example {P R : α → Prop} : (∀ x, P x) ∧ (∀ x, R x) ↔ ∀ x, P x ∧ R x := by
+  exact Iff.symm forall_and
