LeanScratch/LogicProof/FirstOrderLogic/Valuation.lean
@@ -9,8 +9,7 @@ structure Interpretation (TA : TNm → Nat) (PA : PNm → Nat) :=
   funcs : (nm : TNm) → Vec dom (TA nm) → dom
   preds : (nm : PNm) → Vec dom (PA nm) → Prop
 
--- It does not make sense to talk about a valuation without an Interpretation so we inherit
-structure Valuation (TA : TNm → Nat) (PA : PNm → Nat) extends Interpretation TA PA :=
+structure Valuation (TA : TNm → Nat) (PA : PNm → Nat) extends Interpretation TA PA
 
 def Valuation.eval (v : Valuation TA PA) : Term TA → v.dom
   | .const nm args =>
@@ -38,3 +37,69 @@ def Formula.denote (v : Valuation TA PA) : Formula TA PA → Prop
   | .exis b => ∃ x, (b x).denote v
   | .univ b => ∀ x, (b x).denote v
 
+namespace DeBrujin
+
+structure Valuation (TA : TNm → Nat) (PA : PNm → Nat) (n : Nat) extends Interpretation TA PA :=
+  vs : Vec dom n
+
+def Valuation.eval (v : Valuation TA PA n) : Term TA n → v.dom
+  | .var x => v.vs.lookup $ Fin2.ofFin x
+  | .const nm args =>
+      v.funcs nm (mapper args)
+    where
+      mapper {n} : Vec _ n → Vec v.dom n
+        | .nil => .nil
+        | hd %:: tl => v.eval hd %:: mapper tl
+
+def Valuation.assign (base : Valuation TA PA n) (v : base.dom) : Valuation TA PA n.succ :=
+  ⟨base.toInterpretation, v %:: base.vs⟩
+
+def Formula.denote (v : Valuation TA PA n) : Formula TA PA n → Prop
+  -- The additional definition of equality is an unnecacarry addition and should
+  -- be ensured by the user
+  | .pred p args => v.preds p $ args.map v.eval
+
+  | .neg x => ¬x.denote v
+
+  | .disj a b => a.denote v ∨ b.denote v
+  | .conj a b => a.denote v ∧ b.denote v
+
+  | .iff a b => a.denote v ↔ b.denote v
+  | .imp a b => a.denote v → b.denote v
+
+  | .exis b => ∃ x, b.denote (v.assign x)
+  | .univ b => ∀ x, b.denote (v.assign x)
+
+def Term.toHoAS.correct
+    {f : Term TA (0 + n)} {ls : Vec (Term TA 0) n}
+
+    {heq : HEq ls $ ls.map (Valuation.mk interp (%[])).eval}
+
+    : FOL.Valuation.eval ⟨interp⟩ (f.substAll ls).toHoAS
+    = Valuation.eval ⟨interp, ls'⟩ f :=
+  match f with
+  | .var _ => by
+    sorry
+  | .const _ _ => sorry
+
+def Formula.toHoAS.correct
+    {f : Formula TA PA (0 + n)} {ls : Vec (Term TA 0) n}
+
+    {heq : HEq ls $ ls.map (Valuation.mk interp (%[])).eval}
+
+    : (f.substAll ls).toHoAS.denote ⟨interp⟩
+    = f.denote ⟨interp, ls'⟩ :=
+  match f with
+  | .pred p args => by
+    sorry
+
+  | .neg x => sorry
+
+  | .disj a b => sorry
+  | .conj a b => sorry
+
+  | .iff a b => sorry
+  | .imp a b => sorry
+
+  | .exis b => sorry
+  | .univ b => sorry
